src/coq/QCVellvm.v
@@ -8,6 +8,9 @@ From ITree Require Import
      Interp.Recursion
      Events.Exception.
 
+Require Import ExtrOcamlBasic.
+Require Import ExtrOcamlString.
+
 (* TODO: Use the existing vellvm version of this? *)
 Inductive MlResult a e :=
 | MlOk : a -> MlResult a e
@@ -27,15 +30,29 @@ Set Guard Checking.
 Definition interpret (prog : list (toplevel_entity typ (list (block typ)))) : MlResult uvalue string
   := step (TopLevelEnv.interpreter prog).
 
+Axiom to_caml_str : string -> string.
+Extract Constant to_caml_str =>
+"fun (s: char list) ->
+  let r = Bytes.create (List.length s) in
+  let rec fill pos = function
+  | [] -> r
+  | c :: s -> Bytes.set r pos c; fill (pos + 1) s
+  in Bytes.to_string (fill 0 s)".
+
+
+Axiom llc_command : string -> int.
+Extract Constant llc_command => "fun prog -> let f = open_out ""temporary_vellvm.ll"" in Printf.fprintf f ""%s"" prog; close_out f; Sys.command ""clang temporary_vellvm.ll -o vellvmqc && ./vellvmqc""".
+
+Definition run_llc (prog : list (toplevel_entity typ (list (block typ)))) : uvalue
+  := UVALUE_I8 (repr (llc_command (to_caml_str (show prog)))).
+
 Definition always_zeroP (prog : list (toplevel_entity typ (list (block typ)))) : Checker
   := 
     collect (show prog)
-            match interpret prog with
-            | MlOk (UVALUE_I8 x) => checker true
-            | MlError e => checker true (* Ignore errors for now *)
-            | MlOk (UVALUE_IBinop _ _ _) => checker true
-            | MlOk uv => checker true
+            match interpret prog, run_llc prog with
+            | MlOk (UVALUE_I8 x), UVALUE_I8 y => checker (eq x y)
+            | _, _ => checker true
             end.
 
-Extract Constant defNumTests    => "20".
+Extract Constant defNumTests    => "1".
 QuickChick (forAll (run_GenLLVM gen_llvm) always_zeroP).
